<?xml version="1.0"?>
<rdf:RDF xmlns="https://purl.org/net/opt_benchmark#"
     xml:base="https://purl.org/net/opt_benchmark"
     xmlns:dc="http://purl.org/dc/elements/1.1/"
     xmlns:owl="http://www.w3.org/2002/07/owl#"
     xmlns:rdf="http://www.w3.org/1999/02/22-rdf-syntax-ns#"
     xmlns:xml="http://www.w3.org/XML/1998/namespace"
     xmlns:xsd="http://www.w3.org/2001/XMLSchema#"
     xmlns:rdfs="http://www.w3.org/2000/01/rdf-schema#">
    <owl:Ontology rdf:about="https://purl.org/net/opt_benchmark">
        <dc:contributor>Ehecatl Antonio Del Rio Chanona</dc:contributor>
        <dc:contributor>Tom Savage</dc:contributor>
        <dc:creator>Tom Savage</dc:creator>
        <dc:date>14-10-2021</dc:date>
        <dc:description>An ontology to represent optimization problems, solvers, and their solutions.</dc:description>
        <dc:title>Optimization Benchmark Ontology</dc:title>
    </owl:Ontology>
    


    <!-- 
    ///////////////////////////////////////////////////////////////////////////////////////
    //
    // Annotation properties
    //
    ///////////////////////////////////////////////////////////////////////////////////////
     -->

    


    <!-- http://purl.org/dc/elements/1.1/contributor -->

    <owl:AnnotationProperty rdf:about="http://purl.org/dc/elements/1.1/contributor"/>
    


    <!-- http://purl.org/dc/elements/1.1/creator -->

    <owl:AnnotationProperty rdf:about="http://purl.org/dc/elements/1.1/creator"/>
    


    <!-- http://purl.org/dc/elements/1.1/date -->

    <owl:AnnotationProperty rdf:about="http://purl.org/dc/elements/1.1/date"/>
    


    <!-- http://purl.org/dc/elements/1.1/description -->

    <owl:AnnotationProperty rdf:about="http://purl.org/dc/elements/1.1/description"/>
    


    <!-- http://purl.org/dc/elements/1.1/title -->

    <owl:AnnotationProperty rdf:about="http://purl.org/dc/elements/1.1/title"/>
    


    <!-- 
    ///////////////////////////////////////////////////////////////////////////////////////
    //
    // Object Properties
    //
    ///////////////////////////////////////////////////////////////////////////////////////
     -->

    


    <!-- https://purl.org/net/opt_benchmark#has_checkpoint -->

    <owl:ObjectProperty rdf:about="https://purl.org/net/opt_benchmark#has_checkpoint">
        <rdfs:domain rdf:resource="https://purl.org/net/opt_benchmark#opt_solution"/>
        <rdfs:range rdf:resource="https://purl.org/net/opt_benchmark#solution_checkpoint"/>
        <rdfs:comment>Represents an optimization solution having a particular checkpoint in time</rdfs:comment>
        <rdfs:label>Has Checkpoint</rdfs:label>
    </owl:ObjectProperty>
    


    <!-- https://purl.org/net/opt_benchmark#has_constraint -->

    <owl:ObjectProperty rdf:about="https://purl.org/net/opt_benchmark#has_constraint">
        <rdfs:domain rdf:resource="https://purl.org/net/opt_benchmark#opt_constraints"/>
        <rdfs:range rdf:resource="https://purl.org/net/opt_benchmark#opt_constraint"/>
        <rdfs:comment>Represents the relation between a constraint belonging to a set of constraints.</rdfs:comment>
        <rdfs:label>Has Constraint</rdfs:label>
    </owl:ObjectProperty>
    


    <!-- https://purl.org/net/opt_benchmark#has_constraints -->

    <owl:ObjectProperty rdf:about="https://purl.org/net/opt_benchmark#has_constraints">
        <rdfs:domain rdf:resource="https://purl.org/net/opt_benchmark#opt_problem"/>
        <rdfs:range rdf:resource="https://purl.org/net/opt_benchmark#opt_constraints"/>
        <rdfs:comment>Represents the relation between an optimization problem and the set of constraints associated with it.</rdfs:comment>
        <rdfs:label>Has Constraints</rdfs:label>
    </owl:ObjectProperty>
    


    <!-- https://purl.org/net/opt_benchmark#has_function -->

    <owl:ObjectProperty rdf:about="https://purl.org/net/opt_benchmark#has_function">
        <rdfs:domain rdf:resource="https://purl.org/net/opt_benchmark#opt_constraint"/>
        <rdfs:domain rdf:resource="https://purl.org/net/opt_benchmark#opt_objective"/>
        <rdfs:range rdf:resource="https://purl.org/net/opt_benchmark#function"/>
        <rdfs:comment>Represents the relation between a function and either an objective or constraint that has that functional form.</rdfs:comment>
        <rdfs:label>Has Function</rdfs:label>
    </owl:ObjectProperty>
    


    <!-- https://purl.org/net/opt_benchmark#has_objective -->

    <owl:ObjectProperty rdf:about="https://purl.org/net/opt_benchmark#has_objective">
        <rdfs:domain rdf:resource="https://purl.org/net/opt_benchmark#opt_problem"/>
        <rdfs:range rdf:resource="https://purl.org/net/opt_benchmark#opt_objective"/>
        <rdfs:comment>Represents the relation between an optimization problem and it&apos;s objective function</rdfs:comment>
        <rdfs:label>Has Objective</rdfs:label>
    </owl:ObjectProperty>
    


    <!-- https://purl.org/net/opt_benchmark#has_problem -->

    <owl:ObjectProperty rdf:about="https://purl.org/net/opt_benchmark#has_problem">
        <rdfs:domain rdf:resource="https://purl.org/net/opt_benchmark#opt_benchmark"/>
        <rdfs:range rdf:resource="https://purl.org/net/opt_benchmark#opt_problem"/>
        <rdfs:comment>Represents the optimization problem associated to an optimization benchmark.</rdfs:comment>
        <rdfs:label>Has Problem</rdfs:label>
    </owl:ObjectProperty>
    


    <!-- https://purl.org/net/opt_benchmark#has_solution -->

    <owl:ObjectProperty rdf:about="https://purl.org/net/opt_benchmark#has_solution">
        <rdfs:domain rdf:resource="https://purl.org/net/opt_benchmark#opt_benchmark"/>
        <rdfs:range rdf:resource="https://purl.org/net/opt_benchmark#opt_solution"/>
        <rdfs:comment>Represents the solution (itself consisting of a set of checkpoints) associated to an optimization benchmark.</rdfs:comment>
        <rdfs:label>Has Solution</rdfs:label>
    </owl:ObjectProperty>
    


    <!-- https://purl.org/net/opt_benchmark#has_solver -->

    <owl:ObjectProperty rdf:about="https://purl.org/net/opt_benchmark#has_solver">
        <rdfs:domain rdf:resource="https://purl.org/net/opt_benchmark#opt_benchmark"/>
        <rdfs:range rdf:resource="https://purl.org/net/opt_benchmark#opt_solver"/>
        <rdfs:comment>Represents the link between an optimization benchmark and the specific optimization solver that was applied.</rdfs:comment>
        <rdfs:label>Has Solver</rdfs:label>
    </owl:ObjectProperty>
    


    <!-- https://purl.org/net/opt_benchmark#has_variables -->

    <owl:ObjectProperty rdf:about="https://purl.org/net/opt_benchmark#has_variables">
        <rdfs:domain rdf:resource="https://purl.org/net/opt_benchmark#opt_constraint"/>
        <rdfs:domain rdf:resource="https://purl.org/net/opt_benchmark#opt_objective"/>
        <rdfs:range rdf:resource="https://purl.org/net/opt_benchmark#opt_variables"/>
        <rdfs:comment>Represents the link between variables associated to an optimization objective or constraint. This allows constraints and objectives to apply a differing number of variables.</rdfs:comment>
        <rdfs:label>Has Variables</rdfs:label>
    </owl:ObjectProperty>
    


    <!-- 
    ///////////////////////////////////////////////////////////////////////////////////////
    //
    // Data properties
    //
    ///////////////////////////////////////////////////////////////////////////////////////
     -->

    


    <!-- https://purl.org/net/opt_benchmark#continuous_variables -->

    <owl:DatatypeProperty rdf:about="https://purl.org/net/opt_benchmark#continuous_variables">
        <rdfs:domain rdf:resource="https://purl.org/net/opt_benchmark#opt_variables"/>
        <rdfs:range rdf:resource="http://www.w3.org/2001/XMLSchema#integer"/>
        <rdfs:comment>Defines the number of continuous variables within a set of optimization variables.</rdfs:comment>
        <rdfs:label>Continuous Variables</rdfs:label>
    </owl:DatatypeProperty>
    


    <!-- https://purl.org/net/opt_benchmark#discrete_variables -->

    <owl:DatatypeProperty rdf:about="https://purl.org/net/opt_benchmark#discrete_variables">
        <rdfs:domain rdf:resource="https://purl.org/net/opt_benchmark#opt_variables"/>
        <rdfs:range rdf:resource="http://www.w3.org/2001/XMLSchema#integer"/>
        <rdfs:comment>Defines the number of discrete variables within a set of optimization variables.</rdfs:comment>
        <rdfs:label>Discrete Variables</rdfs:label>
    </owl:DatatypeProperty>
    


    <!-- https://purl.org/net/opt_benchmark#has_iteration -->

    <owl:DatatypeProperty rdf:about="https://purl.org/net/opt_benchmark#has_iteration">
        <rdfs:domain rdf:resource="https://purl.org/net/opt_benchmark#solution_checkpoint"/>
        <rdfs:range rdf:resource="http://www.w3.org/2001/XMLSchema#integer"/>
        <rdfs:comment>Defines the iteration at a particular checkpoint.</rdfs:comment>
        <rdfs:label>Has Iteration</rdfs:label>
    </owl:DatatypeProperty>
    


    <!-- https://purl.org/net/opt_benchmark#has_momentum -->

    <owl:DatatypeProperty rdf:about="https://purl.org/net/opt_benchmark#has_momentum">
        <rdfs:domain rdf:resource="https://purl.org/net/opt_benchmark#first_order"/>
        <rdfs:range rdf:resource="http://www.w3.org/2001/XMLSchema#boolean"/>
        <rdfs:comment>Specifies whether the optimization solver includes a momentum term or not.</rdfs:comment>
        <rdfs:label>Has Momentum</rdfs:label>
    </owl:DatatypeProperty>
    


    <!-- https://purl.org/net/opt_benchmark#has_objective_value -->

    <owl:DatatypeProperty rdf:about="https://purl.org/net/opt_benchmark#has_objective_value">
        <rdfs:domain rdf:resource="https://purl.org/net/opt_benchmark#solution_checkpoint"/>
        <rdfs:range rdf:resource="http://www.w3.org/2001/XMLSchema#float"/>
        <rdfs:comment>Represents the value of the objective function at a particular instance.</rdfs:comment>
        <rdfs:label>Has Objective Value</rdfs:label>
    </owl:DatatypeProperty>
    


    <!-- https://purl.org/net/opt_benchmark#has_polynomial_order -->

    <owl:DatatypeProperty rdf:about="https://purl.org/net/opt_benchmark#has_polynomial_order">
        <rdfs:domain rdf:resource="https://purl.org/net/opt_benchmark#polynomial"/>
        <rdfs:range rdf:resource="http://www.w3.org/2001/XMLSchema#integer"/>
        <rdfs:comment>Represents the order or degree of a polynomial</rdfs:comment>
        <rdfs:label>Has Polynomial Order</rdfs:label>
    </owl:DatatypeProperty>
    


    <!-- https://purl.org/net/opt_benchmark#number_of_constraints -->

    <owl:DatatypeProperty rdf:about="https://purl.org/net/opt_benchmark#number_of_constraints">
        <rdfs:domain rdf:resource="https://purl.org/net/opt_benchmark#opt_constraints"/>
        <rdfs:range rdf:resource="http://www.w3.org/2001/XMLSchema#integer"/>
        <rdfs:comment>Represents the integer number of constraints within a set of constraints</rdfs:comment>
        <rdfs:label>Number Of Constraints</rdfs:label>
    </owl:DatatypeProperty>
    


    <!-- 
    ///////////////////////////////////////////////////////////////////////////////////////
    //
    // Classes
    //
    ///////////////////////////////////////////////////////////////////////////////////////
     -->

    


    <!-- https://purl.org/net/opt_benchmark#direct -->

    <owl:Class rdf:about="https://purl.org/net/opt_benchmark#direct">
        <rdfs:subClassOf rdf:resource="https://purl.org/net/opt_benchmark#zero_order"/>
        <rdfs:comment>Direct zero-order methods use direct function evaluations to decide where to move</rdfs:comment>
        <rdfs:label>Direct Zero Order Method</rdfs:label>
    </owl:Class>
    


    <!-- https://purl.org/net/opt_benchmark#equality_constraint -->

    <owl:Class rdf:about="https://purl.org/net/opt_benchmark#equality_constraint">
        <rdfs:subClassOf rdf:resource="https://purl.org/net/opt_benchmark#opt_constraint"/>
        <rdfs:comment>Represents an equality constraint</rdfs:comment>
        <rdfs:label>Equality Constraint</rdfs:label>
    </owl:Class>
    


    <!-- https://purl.org/net/opt_benchmark#first_order -->

    <owl:Class rdf:about="https://purl.org/net/opt_benchmark#first_order">
        <rdfs:subClassOf rdf:resource="https://purl.org/net/opt_benchmark#opt_solver"/>
        <rdfs:comment>First order methods apply only the gradient of a function (i.e. the first derivative)</rdfs:comment>
        <rdfs:label>First Order Method</rdfs:label>
    </owl:Class>
    


    <!-- https://purl.org/net/opt_benchmark#function -->

    <owl:Class rdf:about="https://purl.org/net/opt_benchmark#function">
        <rdfs:comment>A mathematical function</rdfs:comment>
        <rdfs:label>Function</rdfs:label>
    </owl:Class>
    


    <!-- https://purl.org/net/opt_benchmark#inequality_constraint -->

    <owl:Class rdf:about="https://purl.org/net/opt_benchmark#inequality_constraint">
        <rdfs:subClassOf rdf:resource="https://purl.org/net/opt_benchmark#opt_constraint"/>
        <rdfs:comment>Represents an inequality constraint</rdfs:comment>
        <rdfs:label>Inequality Constraint</rdfs:label>
    </owl:Class>
    


    <!-- https://purl.org/net/opt_benchmark#linear -->

    <owl:Class rdf:about="https://purl.org/net/opt_benchmark#linear">
        <rdfs:subClassOf rdf:resource="https://purl.org/net/opt_benchmark#function"/>
        <rdfs:comment>Represents a linear function.</rdfs:comment>
        <rdfs:label>Linear Function</rdfs:label>
    </owl:Class>
    


    <!-- https://purl.org/net/opt_benchmark#model_based -->

    <owl:Class rdf:about="https://purl.org/net/opt_benchmark#model_based">
        <rdfs:subClassOf rdf:resource="https://purl.org/net/opt_benchmark#zero_order"/>
        <rdfs:comment>Model based zero-order optimization methods produce a surrogate, often quadratic, of a function, which at each iteration is optimized.</rdfs:comment>
        <rdfs:label>Model Based Zero Order Method</rdfs:label>
    </owl:Class>
    


    <!-- https://purl.org/net/opt_benchmark#nonlinear -->

    <owl:Class rdf:about="https://purl.org/net/opt_benchmark#nonlinear">
        <rdfs:subClassOf rdf:resource="https://purl.org/net/opt_benchmark#function"/>
        <rdfs:comment>Represents a nonlinear function.</rdfs:comment>
        <rdfs:label>Nonlinear Function</rdfs:label>
    </owl:Class>
    


    <!-- https://purl.org/net/opt_benchmark#opt_benchmark -->

    <owl:Class rdf:about="https://purl.org/net/opt_benchmark#opt_benchmark">
        <rdfs:comment>Represents the combination of an optimization solver, an associated problem, and an associated solution.</rdfs:comment>
        <rdfs:label>Optimization Benchmark</rdfs:label>
    </owl:Class>
    


    <!-- https://purl.org/net/opt_benchmark#opt_constraint -->

    <owl:Class rdf:about="https://purl.org/net/opt_benchmark#opt_constraint">
        <rdfs:comment>Represents a constraint within the set of constraints associated to an optimization problem.</rdfs:comment>
        <rdfs:label>Optimization Constraint</rdfs:label>
    </owl:Class>
    


    <!-- https://purl.org/net/opt_benchmark#opt_constraints -->

    <owl:Class rdf:about="https://purl.org/net/opt_benchmark#opt_constraints">
        <rdfs:comment>Represents the set of contraints associated to an optimization problem or mathematical program.</rdfs:comment>
        <rdfs:label>Optimization Constraints</rdfs:label>
    </owl:Class>
    


    <!-- https://purl.org/net/opt_benchmark#opt_objective -->

    <owl:Class rdf:about="https://purl.org/net/opt_benchmark#opt_objective">
        <rdfs:comment>The objective function (i.e. function to be optimized) of an optimization problem</rdfs:comment>
        <rdfs:label>Optimization Objective</rdfs:label>
    </owl:Class>
    


    <!-- https://purl.org/net/opt_benchmark#opt_problem -->

    <owl:Class rdf:about="https://purl.org/net/opt_benchmark#opt_problem">
        <rdfs:comment>I.e. a mathematical program.</rdfs:comment>
        <rdfs:label>Optimization Problem</rdfs:label>
    </owl:Class>
    


    <!-- https://purl.org/net/opt_benchmark#opt_solution -->

    <owl:Class rdf:about="https://purl.org/net/opt_benchmark#opt_solution">
        <rdfs:subClassOf rdf:resource="https://purl.org/net/opt_benchmark#opt_problem"/>
        <rdfs:comment>Represents the solution that results when an optimization solver is applied to an optimization problem.</rdfs:comment>
        <rdfs:label>Optimization Solution</rdfs:label>
    </owl:Class>
    


    <!-- https://purl.org/net/opt_benchmark#opt_solver -->

    <owl:Class rdf:about="https://purl.org/net/opt_benchmark#opt_solver">
        <rdfs:comment>Represents a solver that solves a mathematical program/optimization problem.</rdfs:comment>
        <rdfs:label>Optimization Solver</rdfs:label>
    </owl:Class>
    


    <!-- https://purl.org/net/opt_benchmark#opt_variables -->

    <owl:Class rdf:about="https://purl.org/net/opt_benchmark#opt_variables">
        <rdfs:comment>Represents the set of variables that a function applies</rdfs:comment>
        <rdfs:label>Optimization Variables</rdfs:label>
    </owl:Class>
    


    <!-- https://purl.org/net/opt_benchmark#polynomial -->

    <owl:Class rdf:about="https://purl.org/net/opt_benchmark#polynomial">
        <rdfs:subClassOf rdf:resource="https://purl.org/net/opt_benchmark#function"/>
        <rdfs:comment>Represents a polynomial function which has a respective degree.</rdfs:comment>
        <rdfs:label>Polynomial Function</rdfs:label>
    </owl:Class>
    


    <!-- https://purl.org/net/opt_benchmark#second_order -->

    <owl:Class rdf:about="https://purl.org/net/opt_benchmark#second_order">
        <rdfs:subClassOf rdf:resource="https://purl.org/net/opt_benchmark#opt_solver"/>
        <rdfs:comment>Second order methods construct a Hessian matrix, or approximation thereof, to guide the next sample.</rdfs:comment>
        <rdfs:label>Second Order Method</rdfs:label>
    </owl:Class>
    


    <!-- https://purl.org/net/opt_benchmark#solution_checkpoint -->

    <owl:Class rdf:about="https://purl.org/net/opt_benchmark#solution_checkpoint">
        <rdfs:comment>Represents the solution at a particular instance within an optimization problem&apos;s solution, in this case, at a specific iterations</rdfs:comment>
        <rdfs:label>Solution Checkpoint</rdfs:label>
    </owl:Class>
    


    <!-- https://purl.org/net/opt_benchmark#zero_order -->

    <owl:Class rdf:about="https://purl.org/net/opt_benchmark#zero_order">
        <rdfs:subClassOf rdf:resource="https://purl.org/net/opt_benchmark#opt_solver"/>
        <rdfs:comment>Zero-order methods do not rely on the use of gradients, also known as derivative-free optimization methods, or black-box optimization methods.</rdfs:comment>
        <rdfs:label>Zero Order Method</rdfs:label>
    </owl:Class>
</rdf:RDF>



<!-- Generated by the OWL API (version 4.5.9.2019-02-01T07:24:44Z) https://github.com/owlcs/owlapi -->

